src/impl/TLS13.Impl.Server.Network.fst
@@ -1304,6 +1304,7 @@ fn process_network_bytes
                    network_out_bytes
                   app_out_bytes /\
                 (buffer_resp.ST.response.ST.status == ST.NeedMoreInput ==>
+                 W.record_prefix_incomplete (Ghost.reveal 'raw_bytes) /\
                  W.parse_record_wire (Ghost.reveal 'raw_bytes) == None /\
                  Seq.equal network_out_bytes (Ghost.reveal 'old_network_out)))
 {
@@ -1331,6 +1332,7 @@ fn process_network_bytes
       assert (pure (buffer_resp.ST.response.ST.status == ST.NeedMoreInput ==>
         buffer_resp.ST.consumed_len == 0sz));
       assert (pure (buffer_resp.ST.response.ST.status == ST.NeedMoreInput ==>
+        W.record_prefix_incomplete (Ghost.reveal 'raw_bytes) /\
         W.parse_record_wire (Ghost.reveal 'raw_bytes) == None));
       assert (pure (buffer_resp.ST.response.ST.status == ST.NeedMoreInput ==>
         Seq.equal (Ghost.reveal 'old_network_out) (Ghost.reveal 'old_network_out)));
