src/impl/TLS13.Impl.Server.fst
@@ -3397,6 +3397,7 @@ fn process_network_bytes
                    network_out_bytes
                    app_out_bytes /\
                 (buffer_resp.ST.response.ST.status == ST.NeedMoreInput ==>
+                  W.record_prefix_incomplete (Ghost.reveal 'raw_bytes) /\
                   W.parse_record_wire (Ghost.reveal 'raw_bytes) == None /\
                   Seq.equal network_out_bytes (Ghost.reveal 'old_network_out)))
 {
@@ -3415,6 +3416,7 @@ fn process_network_bytes
             pts_to network_out network_out_bytes **
             pts_to app_out app_out_bytes);
   assert (pure (buffer_resp.ST.response.ST.status == ST.NeedMoreInput ==>
+    W.record_prefix_incomplete (Ghost.reveal 'raw_bytes) /\
     W.parse_record_wire (Ghost.reveal 'raw_bytes) == None /\
     Seq.equal network_out_bytes (Ghost.reveal 'old_network_out)));
   rewrite (SN.connection_exactly s st1) as (connection_exactly s st1);
